src/program_proof/mvcc/tid_proof.v
@@ -1,17 +1,62 @@
+From Perennial.base_logic Require Import ghost_map saved_prop.
 From Perennial.program_proof.mvcc Require Import mvcc_prelude mvcc_ghost.
 From Goose.github_com.mit_pdos.go_mvcc Require Import tid.
 
 Section program.
 Context `{!heapGS Σ, !mvcc_ghostG Σ}.
 
-Definition have_gentid (γ : mvcc_names) : iProp Σ.
-Admitted.
+Definition gentid_ns := nroot .@ "gentid".
+
+Local Definition gentid_au (γ : mvcc_names) (sid : u64) (Φ : val → iProp Σ) : iProp Σ :=
+  (|NC={⊤ ∖ ∅,∅}=>
+    ∃ ts : nat, ts_auth γ ts ∗
+       ((∃ ts' : nat, ts_auth γ ts' ∗ ⌜(ts < ts')%nat⌝) -∗
+         |NC={∅,⊤ ∖ ∅}=> ∀ tid : u64, ⌜int.nat tid = ts⌝ ∗ sid_own γ sid -∗ Φ #tid)).
+
+Local Definition reserved_inv γ now (ts : u64) γr : iProp Σ :=
+  ∃ Φ, let sid := word.modu ts (U64 N_TXN_SITES) in
+    saved_pred_own γr DfracDiscarded Φ ∗
+    sid_own γ sid ∗
+    if bool_decide (int.nat ts ≤ now)%nat then
+      (* This ts has already happened *)
+      sid_own γ sid -∗ Φ #ts
+    else
+      (* This ts is still in the future *)
+      gentid_au γ sid Φ
+    .
+
+Local Definition gentid_inv (γ : mvcc_names) : iProp Σ :=
+  ∃ now (reserved : gmap u64 gname),
+    ts_auth γ now ∗ tsc_lb now ∗
+    ghost_map_auth γ.(mvcc_gentid_reserved) 1 reserved ∗
+    [∗ map] ts ↦ 'γr ∈ reserved,
+      reserved_inv γ now ts γr.
+
+Definition have_gentid (γ : mvcc_names) : iProp Σ :=
+  inv gentid_ns (gentid_inv γ).
+
+Local Definition tid_reserved γ γr ts (Φ : val → iProp Σ) : iProp Σ :=
+  ghost_map_elem γ.(mvcc_gentid_reserved) ts (DfracOwn 1) γr ∗
+  saved_pred_own γr DfracDiscarded Φ.
 
 Global Instance have_gentid_persistent γ : Persistent (have_gentid γ).
-Proof. Admitted.
+Proof. apply _. Qed.
 
 Lemma init_GenTID γ E :
-  ⊢ |={E}=> have_gentid γ.
+  mvcc_gentid_init γ -∗
+  |={E}=> have_gentid γ.
+Proof. Admitted.
+
+Local Lemma gentid_reserve γ sid Φ :
+  gentid_inv γ -∗
+  sid_own γ sid -∗
+  gentid_au γ sid Φ -∗
+  |==> ∃ clock, tsc_lb clock ∗
+    (* The user can pick a timestamp with the right sid, but only gets something
+    out of this if they pick one that is strictly greater than [clock]. *)
+    (∀ ts, ⌜sid = word.modu ts (U64 N_TXN_SITES)⌝ ==∗
+       (if decide (clock < int.Z ts) then ∃ γr, tid_reserved γ γr ts Φ else True) ∗
+       gentid_inv γ).
 Proof. Admitted.
 
 (**
@@ -29,7 +74,7 @@ Theorem wp_GenTID (sid : u64) γ :
     <<< ∃ ts', ts_auth γ ts' ∗ ⌜(ts < ts')%nat⌝ >>>
     {{{ (tid : u64), RET #tid; ⌜int.nat tid = ts⌝ ∗ sid_own γ sid }}}.
 Proof.
-  iIntros "#Hinv !>" (Φ) "Hpre HAU".
+  iIntros "#Hinv !>" (Φ) "Hsid HAU".
   wp_call.
 
   (***********************************************************)
@@ -37,23 +82,27 @@ Proof.
   (***********************************************************)
   wp_apply wp_ref_of_zero; first done.
   iIntros (tidRef) "Htid".
+  wp_pure1_credit "LC".
   wp_pures.
 
   (***********************************************************)
   (* tid = GetTSC()                                          *)
   (***********************************************************)
-  (* This is a hack *)
-  iMod tsc_lb_0 as "Hlb".
   wp_apply (wp_GetTSC).
-  (* XXX: We're wasting the fupd here since we're not opening any invariant. *)
-  iApply ncfupd_mask_intro; first done.
-  iIntros "HfupdC".
-  iExists 0%nat.
-  iFrame.
-  iIntros (new_time) "[%Hnew Hlb]".
-  iMod "HfupdC".
-  iModIntro.
-  iIntros "_".
+  iInv "Hinv" as "Hgentid" "Hclose".
+  iMod (lc_fupd_elim_later with "LC Hgentid") as "Hgentid".
+  iMod (gentid_reserve with "Hgentid Hsid HAU") as (clock) "[Hclock Hcont]".
+  iApply ncfupd_mask_intro.
+  { solve_ndisj. }
+  iIntros "Hclose2".
+  iExists _. iFrame "Hclock".
+  iIntros (clock2) "[%Hclock Hclock2]".
+  iMod "Hclose2" as "_".
+  set reserved_ts := word.add clock2 (U64 1). (* FIXME use the actual ID here *)
+  iMod ("Hcont" $! reserved_ts with "[]") as "[Hreserved Hgentid]".
+  { iPureIntro. admit. }
+  iMod ("Hclose" with "Hgentid") as "_".
+  iIntros "!> _".
 
   (************************************************************************)
   (* tid = ((tid + config.N_TXN_SITES) & ^(config.N_TXN_SITES - 1)) + sid *)
@@ -81,3 +130,5 @@ Proof.
 Admitted.
 
 End program.
+
+Global Typeclasses Opaque have_gentid.
